specs/Spec.Blake2.fst
@@ -393,13 +393,25 @@ val blake2_update:
   -> kk:size_nat{kk <= 32 /\ (if kk = 0 then length d <= max_limb a else length d + (size_block a) <= max_limb a)} ->
   Tot (hash_ws a)
 
+let spec_update_block 
+    (a:alg) 
+    (init:nat) 
+    (i:nat{init + (i * size_block a) <= max_limb a}) =
+    blake2_update_block a (init + (i * size_block a))
+
+let spec_update_last 
+    (a:alg) 
+    (len:nat{len <= max_limb a})
+    (i:nat) =
+    blake2_update_last a len 
+    
 let blake2_update a s d kk =
   let ll = length d in
   let klen = if kk = 0 then 0 else 1 in
-  let spec_update_block (i:nat{i < ll / (size_block a)}) =
-    blake2_update_block a ((klen + i + 1) * (size_block a)) in
-  let spec_update_last (i:nat) = blake2_update_last a (klen * (size_block a) + ll) in
-  repeati_blocks (size_block a) d spec_update_block spec_update_last s
+  repeati_blocks (size_block a) d 
+    (spec_update_block a ((klen + 1) * size_block a))
+    (spec_update_last a (klen * (size_block a) + ll))
+    s
 
 
 val blake2_finish:
